% Document built on template from Jennifer Pan, http://jenpan.com/jen_pan/PsetLatexTemplate.tex

\documentclass[10pt,letter]{article}
	% basic article document class
	% use percent signs to make comments to yourself -- they will not show up.

\usepackage{amsmath}
\usepackage{amssymb}
	% packages that allow mathematical formatting

\usepackage{graphicx}
	% package that allows you to include graphics

\usepackage{setspace}
	% package that allows you to change spacing

\onehalfspacing
	% text become 1.5 spaced

\usepackage{fullpage}
	% package that specifies normal margins

% Specifying user macros
\newcommand{\matr}[1]{\mathbf{#1}}
\newcommand{\Lagr}{\mathop{\mathcal{L}}}

\begin{document}
	% line of code telling latex that your document is beginning


\title{Linear Algebra Exercises}

\author{Rayhan Momin}

\date{August 2, 2017}
	% Note: when you omit this command, the current dateis automatically included
 
\maketitle 
	% tells latex to follow your header (e.g., title, author) commands.

\section*{Exercise 1}

\begin{flushleft}
Let $x$ be a given $n \times 1$ vector and consider the problem


\[v(x) =  \max_{y,u} \left\{ - y'P y - u' Q u \right\}\]


subject to the linear constraint


\[y = Ax + Bu\]


Here: 


\begin{itemize}
  \item $P$ is an $n \times n$ matrix and $Q$ is an $m \times m$ matrix
  \item $A$ is an $n \times n$ matrix and $B$ is an $n \times m$ matrix
  \item both $P$ and $Q$ are symmetric and positive semidefinite
\end{itemize}


One way to solve this problem is to form the Lagrangian

\[\Lagr = - y' P y - u' Q u + \lambda' \left[A x + B u - y\right]\]


where $\lambda$ is an $n \times 1$ vector of Lagrange multipliers

Show that these conditions imply that

\begin{enumerate}
\item $\lambda = -2Py$
\item The optimizing choice of $u$ satisfies $u = - (Q + B' P B)^{-1} B' P A x$
\item The function $v$ satisfies $v(x) = - x' \tilde P x$ where $\tilde P = A' P A - A'P B (Q + B'P B)^{-1} B' P A$
\end{enumerate}

\end{flushleft}
\section*{My Solution to Exercise 1}

\paragraph{1.}
\begin{align}
  \frac{ \partial \Lagr}{\partial y} & = \frac{ \partial (-y' P y)}{\partial y} - \frac{\partial \lambda' y}{\partial y} & = 0 \\
  & = -(P + P')y - \lambda & = 0 \\
  & = -2Py -\lambda & = 0 \\
  \lambda & = -2Py
\end{align}
\setcounter{equation}{0}

\paragraph{2.}
\begin{align}
  \frac{\partial \Lagr}{\partial u} & = - \frac{\partial(u' Q u)}{\partial u} + \frac{\lambda' B u}{\partial u} & = 0 \\
  & = -(Q +Q')u + (\lambda' B)' \\
  & = -2 Q u + B' \lambda
\end{align}
Recall $\lambda = -2Py$
\begin{align}
  Q u & = -B' P y \\
\end{align}
Recall $y = A x + B u$
\begin{align}
  & = -B' P (A x + B u) \\
  & = -B' P A x - B' P B u \\
  Q u + B' P B u & = -B' P A x \\
  (Q + B' P B)u & = -B' P A x \\
  u & = -(Q + B' P B)^{-1} B' P A x
\end{align}
\setcounter{equation}{0}

\iffalse
\begin{equation} \label{eq:1}
  u = -(Q + B' P B)^{-1} B' P A x
\end{equation}

\begin{equation} \label{eq:2}
  y = A x + B u
\end{equation}

\begin{equation} \label{eq:3}
  v(x) = -y' P y - u' Q u 
\end{equation}
\fi

\paragraph{3.}
Idea is to substitute in $u$ and $y$ into fucntion $v$
\begin{align}
  v(x) & = -y' P y - u' Q u \\
  & = -(A x + B u)' P (A x + B u) - u' Q u
\end{align}
Let $u = - S x$
\begin{align}
  & = -(A x - B S x)' P (A x - B S x) - (S x )' Q S x \\
  & = - \left[ ((A x)' - (B S x)')P(A x - B S x) + (x' S' Q S x) \right] \\
  & = - \left[ (x' A' - x' S' B') (P A x - P B S x) + (x' S' Q S x) \right] \\
  & = - \left[ x' A' P A x - x' S' B' P A x - x' A' P B S x + x' S' B' P B S x +  x' S' Q S x \right]
\end{align}
Note that $S' B' P A$ and $A' P B S$ are symmetric $n \times n$ matrices. $B' P B - Q$ is a symmetric $m \times m$ matrix.

\begin{align}
  & = - x' \left[ A' P A - S' B' P A - (A' P B S)' + S' (B' P B  +  Q)' S \right] x \\
  & = - x' \left[ A' P A - 2 S' B' P A + S' ( Q + B' P B) S \right] x \\
\end{align}
Substitute back in $S = (Q + B' P B)^{-1} B' P A$
\begin{align}
  & = - x' \left[ A' P A - 2 (B' P A)'(Q + B' P B)^{-1}( B' P A) + (B' P A)' (Q + B' P B)^{-1} B' P A \right] x \\
  & = - x' \underbrace{\left[ A' P A - A' P B (Q + B' P B)^{-1} B' P A \right]}_\text{$\tilde P$} x \\
  & = - x' \tilde P x
\end{align}


\end{document}
	% line of code telling latex that your document is ending. If you leave this out, you'll get an error
